Sequences/NatSeqConversions.dfy
@@ -31,7 +31,7 @@ abstract module NatSeqConversions refines NatSeq {
         [NatSeq2.to_nat(xs[..N()]) as NatSeq1.uint] + to_higher_base(xs[N()..])
   }
 
-  lemma lemma_to_lower_base(xs: seq<NatSeq1.uint>)
+  lemma lemma_lower_base_to_nat(xs: seq<NatSeq1.uint>)
     ensures NatSeq2.to_nat(to_lower_base(xs)) == NatSeq1.to_nat(xs)
   {
     reveal NatSeq1.to_nat();
@@ -47,7 +47,7 @@ abstract module NatSeqConversions refines NatSeq {
           {
             NatSeq2.lemma_to_seq_with_len_eq_to_seq(first(xs), N());
             NatSeq2.lemma_nat_seq_nat(first(xs));
-            lemma_to_lower_base(drop_first(xs));
+            lemma_lower_base_to_nat(drop_first(xs));
           }
         first(xs) + NatSeq1.to_nat(drop_first(xs)) * power(NatSeq2.BASE(), N());
           { assert power(NatSeq2.BASE(), N()) == NatSeq1.BASE(); }
@@ -56,7 +56,7 @@ abstract module NatSeqConversions refines NatSeq {
     }
   }
 
-  lemma lemma_to_higher_base(xs: seq<NatSeq2.uint>)
+  lemma lemma_higher_base_to_nat(xs: seq<NatSeq2.uint>)
     ensures NatSeq1.to_nat(to_higher_base(xs)) == NatSeq2.to_nat(xs)
   {
     reveal NatSeq1.to_nat();
@@ -68,12 +68,58 @@ abstract module NatSeqConversions refines NatSeq {
           { NatSeq2.lemma_seq_nat_bound(xs[..N()]); }
         NatSeq1.to_nat([NatSeq2.to_nat(xs[..N()]) as NatSeq1.uint] + to_higher_base(xs[N()..]));
         NatSeq2.to_nat(xs[..N()]) as NatSeq1.uint + NatSeq1.to_nat(to_higher_base(xs[N()..])) * NatSeq1.BASE();
-          { lemma_to_higher_base(xs[N()..]); }
+          { lemma_higher_base_to_nat(xs[N()..]); }
         NatSeq2.to_nat(xs[..N()]) + NatSeq2.to_nat(xs[N()..]) * power(NatSeq2.BASE(), N());
           { NatSeq2.lemma_seq_prefix(xs, N()); }
         NatSeq2.to_nat(xs);
       }
     }
+  }
+
+  lemma lemma_to_lower_base_is_injective(xs: seq<NatSeq1.uint>,
+                                         ys: seq<NatSeq1.uint>)
+    requires |xs| == |ys|
+    requires NatSeq1.to_nat(xs) == NatSeq1.to_nat(ys)
+    ensures to_lower_base(xs) == to_lower_base(ys)
+  {
+    calc ==> {
+      to_lower_base(xs) != to_lower_base(ys);
+        { NatSeq1.lemma_seq_neq(xs, ys, |xs|); }
+      NatSeq1.to_nat(xs) != NatSeq1.to_nat(ys);
+      false;
+    }
+  }
+
+  lemma lemma_to_higher_base_is_injective(xs: seq<NatSeq2.uint>,
+                                          ys: seq<NatSeq2.uint>)
+    requires |xs| == |ys|
+    requires NatSeq2.to_nat(xs) == NatSeq2.to_nat(ys)
+    ensures to_higher_base(xs) == to_higher_base(ys)
+  {
+    calc ==> {
+      to_higher_base(xs) != to_higher_base(ys);
+        { NatSeq2.lemma_seq_neq(xs, ys, |xs|); }
+      NatSeq2.to_nat(xs) != NatSeq2.to_nat(ys);
+      false;
+    }
+  }
+
+  lemma lemma_to_lower_base_is_injective_inv(xs: seq<NatSeq1.uint>,
+                                             ys: seq<NatSeq1.uint>)
+    requires to_lower_base(xs) == to_lower_base(ys)
+    ensures NatSeq1.to_nat(xs) == NatSeq1.to_nat(ys)
+  {
+    lemma_lower_base_to_nat(xs);
+    lemma_lower_base_to_nat(ys);
+  }
+
+  lemma lemma_to_higher_base_is_injective_inv(xs: seq<NatSeq2.uint>,
+                                              ys: seq<NatSeq2.uint>)
+    requires to_higher_base(xs) == to_higher_base(ys)
+    ensures NatSeq2.to_nat(xs) == NatSeq2.to_nat(ys)
+  {
+    lemma_higher_base_to_nat(xs);
+    lemma_higher_base_to_nat(ys);
   }
 
 }
